

A cool proof [1]:

$$V_0(0) = \frac{1}{1+R} [q_0^1(0)V_1(1) + q_0^0(0)V_1(0)],$$

of the theorem:

$$\begin{aligned} V_0(0) &= \frac{M}{(1+R)^N} \sum_{j=0}^{2^N-1} e^{\beta-1} \sum_{k=0}^{N-1} \alpha_k(\lfloor j/2^{N-k} \rfloor) \\ &\quad \Phi(Su^{r_N(j)}d^{N-r_N(j)}) \prod_{k=1}^N q_{k-1}^{\text{mod}(\lfloor j/2^{N-k} \rfloor, 2)}(\lfloor j/2^{N-(k-1)} \rfloor) = \\ &\quad \frac{1}{(1+R)^N} \sum_{j=0}^{2^N-1} V_N(j) \prod_{k=1}^N q_{k-1}^{\text{mod}(\lfloor j/2^{N-k} \rfloor, 2)}(\lfloor j/2^{N-(k-1)} \rfloor). \end{aligned}$$

[1] Gerardo Hernández-del-Valle, Explicit formulae for the valuation of European options with price impacts, 2025. <https://www.sciencedirect.com/science/article/pii/S2405918824000187>